theories/int_or_ptr/vst/verif/vsu.v
@@ -7,14 +7,14 @@ From appliedfm Require Import int_or_ptr.vst.verif.verif.
 
 #[local] Existing Instance NullExtension.Espec.
 
-Lemma int_or_ptr__vsu: VSU [] int_or_ptr__specs.imports ltac:(QPprog prog) int_or_ptr__specs.exports emp.
+Lemma int_or_ptr__vsu: VSU int_or_ptr__specs.externs int_or_ptr__specs.imports ltac:(QPprog prog) int_or_ptr__specs.exports emp.
 Proof.
-mkVSU prog int_or_ptr__specs.all.
-- solve_SF_internal body_int_or_ptr__sizeof.
-- solve_SF_internal body_int_or_ptr__alignof.
-- solve_SF_internal body_int_or_ptr__is_int.
-- solve_SF_internal body_int_or_ptr__to_int.
-- solve_SF_internal body_int_or_ptr__to_ptr.
-- solve_SF_internal body_int_or_ptr__of_int.
-- solve_SF_internal body_int_or_ptr__of_ptr.
+  mkVSU prog int_or_ptr__specs.all.
+  - solve_SF_internal body_int_or_ptr__sizeof.
+  - solve_SF_internal body_int_or_ptr__alignof.
+  - solve_SF_internal body_int_or_ptr__is_int.
+  - solve_SF_internal body_int_or_ptr__to_int.
+  - solve_SF_internal body_int_or_ptr__to_ptr.
+  - solve_SF_internal body_int_or_ptr__of_int.
+  - solve_SF_internal body_int_or_ptr__of_ptr.
 Qed.
